factor-out trusted parts of main.dfy from untrusted proofs

verified/main.dfy
@@ -1,334 +1,36 @@
-include "ARMprint.s.dfy"
-include "smc_handler.gen.dfy"
-include "exception_handlers.gen.dfy"
+include "exhandler_state.i.dfy"
 
-function method smc_handler():va_code  { va_code_smc_handler() }
-function method svc_handler():va_code  { va_code_svc_handler() }
-function method abt_handler():va_code  { va_code_abort_handler(ExAbt) }
-function method und_handler():va_code  { va_code_abort_handler(ExUnd) }
-function method fiq_handler():va_code  { va_code_interrupt_handler(ExFIQ) }
-function method irq_handler():va_code  { va_code_interrupt_handler(ExIRQ) }
-
-method printExceptionHandlerReturn()
-{
-    printInsFixed("B", user_continue_label());
-}
-
-method printInterruptHandlerReturn()
-{
-    printIns2Op("TST", OSP, OConst(1));
-    printInsFixed("BNE", user_continue_label());
-    printInsFixed("MOVS", "pc, lr");
-}
-
-method printSMCHandlerReturn()
-{
-    printInsFixed("MOVS", "pc, lr");
-}
-
-method printKSHA256()
-{
-    print(".type g_k_sha256, %object"); nl();
-    print(".align 5"); nl();
-    print("g_k_sha256:"); nl();
-    print(".word 0x428a2f98,0x71374491,0xb5c0fbcf,0xe9b5dba5"); nl();
-    print(".word 0x3956c25b,0x59f111f1,0x923f82a4,0xab1c5ed5"); nl();
-    print(".word 0xd807aa98,0x12835b01,0x243185be,0x550c7dc3"); nl();
-    print(".word 0x72be5d74,0x80deb1fe,0x9bdc06a7,0xc19bf174"); nl();
-    print(".word 0xe49b69c1,0xefbe4786,0x0fc19dc6,0x240ca1cc"); nl();
-    print(".word 0x2de92c6f,0x4a7484aa,0x5cb0a9dc,0x76f988da"); nl();
-    print(".word 0x983e5152,0xa831c66d,0xb00327c8,0xbf597fc7"); nl();
-    print(".word 0xc6e00bf3,0xd5a79147,0x06ca6351,0x14292967"); nl();
-    print(".word 0x27b70a85,0x2e1b2138,0x4d2c6dfc,0x53380d13"); nl();
-    print(".word 0x650a7354,0x766a0abb,0x81c2c92e,0x92722c85"); nl();
-    print(".word 0xa2bfe8a1,0xa81a664b,0xc24b8b70,0xc76c51a3"); nl();
-    print(".word 0xd192e819,0xd6990624,0xf40e3585,0x106aa070"); nl();
-    print(".word 0x19a4c116,0x1e376c08,0x2748774c,0x34b0bcb5"); nl();
-    print(".word 0x391c0cb3,0x4ed8aa4a,0x5b9cca4f,0x682e6ff3"); nl();
-    print(".word 0x748f82ee,0x78a5636f,0x84c87814,0x8cc70208"); nl();
-    print(".word 0x90befffa,0xa4506ceb,0xbef9a3f7,0xc67178f2"); nl();
-    print(".size g_k_sha256,.-g_k_sha256"); nl();
-    print(".word 0   @ terminator"); nl();
-}
-
-// TODO: clean this up (or move it to the loader)
-method printStack()
-{
-    print(".align 3"); nl(); // 8-byte alignment
-    print(".global monitor_stack_base"); nl();
-    print("monitor_stack_limit:"); nl();
-    print(".skip "); print(KOM_STACK_SIZE); nl();
-    print("monitor_stack_base:"); nl();
-}
-
-method printAll()
-{
-    var n := 0;
-    var monitor_vectbl := emptyVecTbl().(
-        svc_smc := Just("smc"),
-        fiq := Just("fiq"),
-        irq := Just("irq"));
-    var secure_vectbl := emptyVecTbl().(
-        undef := Just("undefined"),
-        svc_smc := Just("svc"),
-        prefetch_abort := Just("abort"),
-        data_abort := Just("abort"));
-
-    printHeader(); nl();
-
-    print(".section vectors, \"ax\""); nl();
-    printVecTbl("_monitor_vectors", monitor_vectbl); nl();
-    printVecTbl("_secure_vectors", secure_vectbl); nl();
-
-    nl();
-    print(".section .text"); nl();
-
-    n := printFunction("abort", abt_handler(), n);
-    printExceptionHandlerReturn(); nl();
-
-    n := printFunction("undefined", und_handler(), n);
-    printExceptionHandlerReturn(); nl();
-
-    n := printFunction("svc", svc_handler(), n);
-    printExceptionHandlerReturn(); nl();
-
-    n := printFunction("smc", smc_handler(), n);
-    printSMCHandlerReturn(); nl();
-
-    n := printFunction("fiq", fiq_handler(), n);
-    printInterruptHandlerReturn(); nl();
-
-    n := printFunction("irq", irq_handler(), n);
-    printInterruptHandlerReturn(); nl();
-
-    nl(); print(".section .data"); nl();
-    printKSHA256(); nl();
-
-    var bssglobals
-        := map o | o in KomGlobalDecls() && o != K_SHA256s() :: KomGlobalDecls()[o];
-    print(".global g_monitor_physbase, g_secure_physbase"); nl();
-    printBss(bssglobals);
-    printStack();
-
-    printFooter();
-}
-
-// these are global assumptions
-predicate GlobalAssumptions()
-{
-    SaneConstants()
-        && UsermodeContinuationPreconditionDef()
-        && UsermodeContinuationInvariantDef()
-        && InterruptContinuationPreconditionDef()
-        && InterruptContinuationInvariantDef()
-}
-
-// this is what we assume about the initial state on entry to the SMC handler
-predicate InitialSMCState(s:state)
-{
-    reveal ValidRegState();
-    reveal ValidSRegState();
-
-    ValidState(s) && s.ok
-        && SaneMem(s.m)
-        && mode_of_state(s) == Monitor
-        && s.conf.scr.ns == NotSecure
-        && !interrupts_enabled(s)
-        && s.regs[SP(Monitor)] == StackBase()
-        && decode_psr(s.sregs[spsr(Monitor)]).m != Monitor
-}
-
-function exHandler(ex:exception): va_code
-{
-    match ex
-        case ExAbt => abt_handler()
-        case ExUnd => und_handler()
-        case ExSVC => svc_handler()
-        case ExFIQ => fiq_handler()
-        case ExIRQ => irq_handler()
-}
-
-lemma lemma_KomUserEntryPrecond_AbsPT(s:state, pagedb:PageDb, dispPg:PageNr)
-    requires KomUserEntryPrecondition(s, pagedb, dispPg)
-    ensures ExtractAbsPageTable(s).Just?
-{
-    lemma_ptablesmatch(s.m, pagedb, l1pOfDispatcher(pagedb, dispPg));
-}
-
-predicate ExceptionStateSideEffects(s:state)
-{
-    ValidState(s) && mode_of_state(s) != User
-    && if s.conf.ex == ExFIQ || s.conf.ex == ExIRQ
-        then mode_of_state(s) == Monitor && !interrupts_enabled(s)
-    else
-        interrupts_enabled(s) &&
-        mode_of_state(s) == (match s.conf.ex
-            case ExAbt => Abort
-            case ExUnd => Undefined
-            case ExSVC => Supervisor)
-}
-
-lemma lemma_KomUserEntryPrecond_Preserved(s0:state, s2:state, r:state,
-                                          pagedb0:PageDb, dispPg:PageNr)
-                                          returns (pagedb: PageDb)
-    requires KomUserEntryPrecondition(s0, pagedb0, dispPg)
-    requires evalUserExecution(s0, s2, r)
-    ensures pagedb == updateUserPagesFromState(r, pagedb0, dispPg)
-    ensures KomUserEntryPrecondition(r, pagedb, dispPg)
-{
-    lemma_KomUserEntryPrecond_AbsPT(s0, pagedb0, dispPg);
-    lemma_userExecutionModel_validity(s0, s2, r);
-    lemma_userExecutionPreservesPrivState(s0, r);
-    lemma_userExecutionUpdatesPageDb(pagedb0, s0, r, dispPg);
-    lemma_executionPreservesMasks(s0, r);
-
-    pagedb := updateUserPagesFromState(r, pagedb0, dispPg);
-    assert l1pOfDispatcher(pagedb, dispPg) == l1pOfDispatcher(pagedb0, dispPg)
-        && finalDispatcher(pagedb, dispPg)
-        by { reveal updateUserPagesFromState(); }
-}
-
-lemma lemma_UserExceptionStateSideEffects(s0:state, s2:state, r:state,
-                                          pagedb0:PageDb, dispPg:PageNr)
-    requires KomUserEntryPrecondition(s0, pagedb0, dispPg)
-    requires evalUserExecution(s0, s2, r)
-    ensures ExceptionStateSideEffects(r) && spsr_of_state(r).m == User
-    ensures !spsr_of_state(r).f && !spsr_of_state(r).i
-{
-    lemma_KomUserEntryPrecond_AbsPT(s0, pagedb0, dispPg);
-    assert evalEnterUserspace(s0, s2);
-    assert mode_of_state(s2) == User;
-    assert s2.conf.scr == s0.conf.scr == SCRT(Secure, true, true);
-    lemma_evalEnterUserspace_preservesAbsPageTable(s0, s2);
-    lemma_userExecutionModel_validity(s0, s2, r);
-    lemma_userExecutionPreservesPrivState(s0, r);
-    lemma_executionPreservesMasks(s0, r);
-
-    var (s3, expc, ex) := userspaceExecutionFn(s2, OperandContents(s0, OLR));
-    assert mode_of_state(s3) == mode_of_state(s2) == User
-        && s3.conf.scr == s2.conf.scr
-        by { reveal userspaceExecutionFn(); }
-
-    assert evalExceptionTaken(s3, ex, expc, r);
-    assert r.conf.ex == ex;
-    lemma_evalExceptionTaken_Mode(s3, ex, expc, r);
-    assert spsr_of_state(r).m == mode_of_state(s3) == User;
-    if ex == ExFIQ || ex == ExIRQ {
-        assert mode_of_state(r) == Monitor;
-        mode_encodings_are_sane();
-        lemma_update_psr(cpsr_of_state(s3), encode_mode(Monitor), true, true);
-        assert !interrupts_enabled(r);
-    } else {
-        assert mode_of_state(r) != Monitor;
-        assert ex != ExFIQ;
-        assert !s3.conf.cpsr.f by
-            { reveal userspaceExecutionFn(); }
-        lemma_update_psr(cpsr_of_state(s3),
-            encode_mode(mode_of_state(r)), false, true);
-        assert !r.conf.cpsr.f;
-        assert interrupts_enabled(r);
-    }
-    assert ExceptionStateSideEffects(r);
-}
-
-lemma lemma_PrivExceptionStateSideEffects(s:state, r:state, ex:exception,
-                                          pagedb:PageDb, dispPg:PageNr)
-    requires KomUserEntryPrecondition(s, pagedb, dispPg)
-    requires priv_of_state(s) == PL1 && interrupts_enabled(s)
-    requires ex == ExIRQ || ex == ExFIQ
-    requires evalExceptionTaken(s, ex, nondet_word(s.conf.nondet, NONDET_PC()), r)
-    ensures ExceptionStateSideEffects(r) && spsr_of_state(r).m == mode_of_state(s)
-{
-    assert r.conf.ex == ex;
-    lemma_evalExceptionTaken_Mode(s, ex, nondet_word(s.conf.nondet, NONDET_PC()), r);
-    assert spsr_of_state(r).m == mode_of_state(s);
-    assert mode_of_state(r) == Monitor;
-    mode_encodings_are_sane();
-    lemma_update_psr(cpsr_of_state(s), encode_mode(Monitor), true, true);
-    assert !interrupts_enabled(r);
-}
-
-lemma lemma_evalHandler(s:state, r:state, pagedb:PageDb, dispPg: PageNr)
-    requires GlobalAssumptions() && ExceptionStateSideEffects(s)
-    requires KomUserEntryPrecondition(s, pagedb, dispPg) && mode_of_state(s) != User
-    requires evalCode(exHandler(s.conf.ex), s, r)
-    requires spsr_of_state(s).m == User // proofs about PL1 interrupts go elsewhere
-    requires !(s.conf.ex == ExIRQ || s.conf.ex == ExFIQ) ==>
-        !spsr_of_state(s).f && !spsr_of_state(s).i
-    ensures KomExceptionHandlerInvariant(s, pagedb, r, dispPg)
-{
-    var block := va_CCons(exHandler(s.conf.ex), va_CNil());
-    reveal va_eval();
-    assert va_eval(Block(block), s, r) by { assert evalBlock(block, s, r); }
-    if s.conf.ex == ExIRQ || s.conf.ex == ExFIQ {
-        var _, _, p := va_lemma_interrupt_handler(block, s, r, s.conf.ex, pagedb, dispPg);
-    } else if s.conf.ex == ExAbt || s.conf.ex == ExUnd {
-        var _, _, p := va_lemma_abort_handler(block, s, r, s.conf.ex, pagedb, dispPg);
-    } else if s.conf.ex == ExSVC {
-        var _, _, p := va_lemma_svc_handler(block, s, r, pagedb, dispPg);
-    }
-}
-
-lemma lemma_SMCHandlerIsCorrect()
+method Main()
+    requires GlobalAssumptions()
 {
     // prove that the SMC handler is correct
     forall s1:state, p1:PageDb, s2:state
-        | GlobalAssumptions() && InitialSMCState(s1)
-        && validPageDb(p1) && pageDbCorresponds(s1.m, p1)
+        | InitialSMCState(s1) && validPageDb(p1) && pageDbCorresponds(s1.m, p1)
         && evalCode(smc_handler(), s1, s2)
         ensures exists p2:PageDb :: smchandler(s1, p1, s2, p2)
             && validPageDb(p2) && pageDbCorresponds(s2.m, p2)
-    {
-        var stack_bytes := KOM_STACK_SIZE - WORDSIZE;
-        assert StackBytesRemaining(s1, stack_bytes);
-        reveal va_eval();
-        var block := va_CCons(smc_handler(), va_CNil());
-        assert va_eval(Block(block), s1, s2) by { assert evalBlock(block, s1, s2); }
-        var _, _, p2' := va_lemma_smc_handler(block, s1, s2, stack_bytes, p1);
-        assert smchandler(s1, p1, s2, p2');
-        assert validPageDb(p2') && pageDbCorresponds(s2.m, p2');
-    }
-}
+    { lemma_SMCHandlerIsCorrect(s1, p1, s2); }
 
-lemma lemma_ExceptionHandlersAreCorrect()
-{
     // prove that whenever we take an exception from user mode, we can run the right
     // handler and it will establish the invariants assumed in the SMC path
     forall s0:state, s1:state, s3:state, r:state
-        | GlobalAssumptions() && ValidState(s0) && s0.ok
+        | ValidState(s0) && s0.ok
         && UsermodeContinuationPrecondition(s0)
         && evalUserExecution(s0, s1, s3)
         && evalCode(exHandler(s3.conf.ex), s3, r)
         ensures exists p2, dp :: KomExceptionHandlerInvariant(s3, p2, r, dp)
-    {
-        var pagedb, dispPg := lemma_UsermodeContinuationPreconditionDef(s0);
-        assert KomUserEntryPrecondition(s0, pagedb, dispPg);
-        lemma_UserExceptionStateSideEffects(s0, s1, s3, pagedb, dispPg);
-        var pagedb' := lemma_KomUserEntryPrecond_Preserved(s0, s1, s3, pagedb, dispPg);
-        lemma_evalHandler(s3, r, pagedb', dispPg);
-    }
+    { lemma_UserModeExceptionHandlersAreCorrect(s0, s1, s3, r); }
 
     // prove that interrupts taken from PL1 modes maintain the invariant
     forall s0:state, ex:exception, s1:state, r:state
-        | GlobalAssumptions() && ValidState(s0) && s0.ok
+        | ValidState(s0) && s0.ok
         && UsermodeContinuationPrecondition(s0)
         && priv_of_state(s0) == PL1 && interrupts_enabled(s0)
         && (ex == ExFIQ || ex == ExIRQ)
         && evalExceptionTaken(s0, ex, nondet_word(s0.conf.nondet, NONDET_PC()), s1)
         && evalCode(exHandler(ex), s1, r)
         ensures exists p0, dp :: KomInterruptHandlerInvariant(s1, p0, r, dp)
-    {
-        var pagedb, dispPg := lemma_UsermodeContinuationPreconditionDef(s0);
-        lemma_PrivExceptionStateSideEffects(s0, s1, ex, pagedb, dispPg);
-        reveal va_eval();
-        var block := va_CCons(exHandler(ex), va_CNil());
-        assert va_eval(Block(block), s1, r) by { assert evalBlock(block, s1, r); }
-        var _, _, p := va_lemma_interrupt_handler(block, s1, r, ex, pagedb, dispPg);
-        assert KomInterruptHandlerInvariant(s1, pagedb, r, dispPg);
-    }
-}
+    { lemma_PrivModeExceptionHandlersAreCorrect(s0, ex, s1, r); }
 
-method Main()
-{
     printAll();
 }
