verified/exhandler_state.i.dfy
@@ -1,0 +1,175 @@
+include "exhandler_state.s.dfy"
+
+lemma lemma_KomUserEntryPrecond_AbsPT(s:state, pagedb:PageDb, dispPg:PageNr)
+    requires KomUserEntryPrecondition(s, pagedb, dispPg)
+    ensures ExtractAbsPageTable(s).Just?
+{
+    lemma_ptablesmatch(s.m, pagedb, l1pOfDispatcher(pagedb, dispPg));
+}
+
+predicate ExceptionStateSideEffects(s:state)
+{
+    ValidState(s) && mode_of_state(s) != User
+    && if s.conf.ex == ExFIQ || s.conf.ex == ExIRQ
+        then mode_of_state(s) == Monitor && !interrupts_enabled(s)
+    else
+        interrupts_enabled(s) &&
+        mode_of_state(s) == (match s.conf.ex
+            case ExAbt => Abort
+            case ExUnd => Undefined
+            case ExSVC => Supervisor)
+}
+
+lemma lemma_KomUserEntryPrecond_Preserved(s0:state, s2:state, r:state,
+                                          pagedb0:PageDb, dispPg:PageNr)
+                                          returns (pagedb: PageDb)
+    requires KomUserEntryPrecondition(s0, pagedb0, dispPg)
+    requires evalUserExecution(s0, s2, r)
+    ensures pagedb == updateUserPagesFromState(r, pagedb0, dispPg)
+    ensures KomUserEntryPrecondition(r, pagedb, dispPg)
+{
+    lemma_KomUserEntryPrecond_AbsPT(s0, pagedb0, dispPg);
+    lemma_userExecutionModel_validity(s0, s2, r);
+    lemma_userExecutionPreservesPrivState(s0, r);
+    lemma_userExecutionUpdatesPageDb(pagedb0, s0, r, dispPg);
+    lemma_executionPreservesMasks(s0, r);
+
+    pagedb := updateUserPagesFromState(r, pagedb0, dispPg);
+    assert l1pOfDispatcher(pagedb, dispPg) == l1pOfDispatcher(pagedb0, dispPg)
+        && finalDispatcher(pagedb, dispPg)
+        by { reveal updateUserPagesFromState(); }
+}
+
+lemma lemma_UserExceptionStateSideEffects(s0:state, s2:state, r:state,
+                                          pagedb0:PageDb, dispPg:PageNr)
+    requires KomUserEntryPrecondition(s0, pagedb0, dispPg)
+    requires evalUserExecution(s0, s2, r)
+    ensures ExceptionStateSideEffects(r) && spsr_of_state(r).m == User
+    ensures !spsr_of_state(r).f && !spsr_of_state(r).i
+{
+    lemma_KomUserEntryPrecond_AbsPT(s0, pagedb0, dispPg);
+    assert evalEnterUserspace(s0, s2);
+    assert mode_of_state(s2) == User;
+    assert s2.conf.scr == s0.conf.scr == SCRT(Secure, true, true);
+    lemma_evalEnterUserspace_preservesAbsPageTable(s0, s2);
+    lemma_userExecutionModel_validity(s0, s2, r);
+    lemma_userExecutionPreservesPrivState(s0, r);
+    lemma_executionPreservesMasks(s0, r);
+
+    var (s3, expc, ex) := userspaceExecutionFn(s2, OperandContents(s0, OLR));
+    assert mode_of_state(s3) == mode_of_state(s2) == User
+        && s3.conf.scr == s2.conf.scr
+        by { reveal userspaceExecutionFn(); }
+
+    assert evalExceptionTaken(s3, ex, expc, r);
+    assert r.conf.ex == ex;
+    lemma_evalExceptionTaken_Mode(s3, ex, expc, r);
+    assert spsr_of_state(r).m == mode_of_state(s3) == User;
+    if ex == ExFIQ || ex == ExIRQ {
+        assert mode_of_state(r) == Monitor;
+        mode_encodings_are_sane();
+        lemma_update_psr(cpsr_of_state(s3), encode_mode(Monitor), true, true);
+        assert !interrupts_enabled(r);
+    } else {
+        assert mode_of_state(r) != Monitor;
+        assert ex != ExFIQ;
+        assert !s3.conf.cpsr.f by
+            { reveal userspaceExecutionFn(); }
+        lemma_update_psr(cpsr_of_state(s3),
+            encode_mode(mode_of_state(r)), false, true);
+        assert !r.conf.cpsr.f;
+        assert interrupts_enabled(r);
+    }
+    assert ExceptionStateSideEffects(r);
+}
+
+lemma lemma_PrivExceptionStateSideEffects(s:state, r:state, ex:exception,
+                                          pagedb:PageDb, dispPg:PageNr)
+    requires KomUserEntryPrecondition(s, pagedb, dispPg)
+    requires priv_of_state(s) == PL1 && interrupts_enabled(s)
+    requires ex == ExIRQ || ex == ExFIQ
+    requires evalExceptionTaken(s, ex, nondet_word(s.conf.nondet, NONDET_PC()), r)
+    ensures ExceptionStateSideEffects(r) && spsr_of_state(r).m == mode_of_state(s)
+{
+    assert r.conf.ex == ex;
+    lemma_evalExceptionTaken_Mode(s, ex, nondet_word(s.conf.nondet, NONDET_PC()), r);
+    assert spsr_of_state(r).m == mode_of_state(s);
+    assert mode_of_state(r) == Monitor;
+    mode_encodings_are_sane();
+    lemma_update_psr(cpsr_of_state(s), encode_mode(Monitor), true, true);
+    assert !interrupts_enabled(r);
+}
+
+lemma lemma_evalHandler(s:state, r:state, pagedb:PageDb, dispPg: PageNr)
+    requires GlobalAssumptions() && ExceptionStateSideEffects(s)
+    requires KomUserEntryPrecondition(s, pagedb, dispPg) && mode_of_state(s) != User
+    requires evalCode(exHandler(s.conf.ex), s, r)
+    requires spsr_of_state(s).m == User // proofs about PL1 interrupts go elsewhere
+    requires !(s.conf.ex == ExIRQ || s.conf.ex == ExFIQ) ==>
+        !spsr_of_state(s).f && !spsr_of_state(s).i
+    ensures KomExceptionHandlerInvariant(s, pagedb, r, dispPg)
+{
+    var block := va_CCons(exHandler(s.conf.ex), va_CNil());
+    reveal va_eval();
+    assert va_eval(Block(block), s, r) by { assert evalBlock(block, s, r); }
+    if s.conf.ex == ExIRQ || s.conf.ex == ExFIQ {
+        var _, _, p := va_lemma_interrupt_handler(block, s, r, s.conf.ex, pagedb, dispPg);
+    } else if s.conf.ex == ExAbt || s.conf.ex == ExUnd {
+        var _, _, p := va_lemma_abort_handler(block, s, r, s.conf.ex, pagedb, dispPg);
+    } else if s.conf.ex == ExSVC {
+        var _, _, p := va_lemma_svc_handler(block, s, r, pagedb, dispPg);
+    }
+}
+
+lemma lemma_SMCHandlerIsCorrect(s1:state, p1:PageDb, s2:state)
+    requires GlobalAssumptions() && InitialSMCState(s1)
+        && validPageDb(p1) && pageDbCorresponds(s1.m, p1)
+        && evalCode(smc_handler(), s1, s2)
+    ensures exists p2 :: smchandler(s1, p1, s2, p2)
+            && validPageDb(p2) && SaneMem(s2.m) && pageDbCorresponds(s2.m, p2)
+{
+    var stack_bytes := KOM_STACK_SIZE - WORDSIZE;
+    assert StackBytesRemaining(s1, stack_bytes);
+    reveal va_eval();
+    var block := va_CCons(smc_handler(), va_CNil());
+    assert va_eval(Block(block), s1, s2) by { assert evalBlock(block, s1, s2); }
+    var _, _, p2' := va_lemma_smc_handler(block, s1, s2, stack_bytes, p1);
+    assert smchandler(s1, p1, s2, p2');
+    assert validPageDb(p2') && pageDbCorresponds(s2.m, p2');
+}
+
+lemma lemma_UserModeExceptionHandlersAreCorrect(s0:state, s1:state, s3:state, r:state)
+    requires GlobalAssumptions() && ValidState(s0) && s0.ok
+        && UsermodeContinuationPrecondition(s0)
+        && evalUserExecution(s0, s1, s3)
+        && evalCode(exHandler(s3.conf.ex), s3, r)
+    ensures mode_of_state(s3) != User && SaneMem(s3.m)
+    ensures exists p2, dp:PageNr :: validPageDb(p2) && pageDbCorresponds(s3.m, p2)
+        && finalDispatcher(p2, dp) && KomExceptionHandlerInvariant(s3, p2, r, dp)
+{
+    var pagedb, dispPg := lemma_UsermodeContinuationPreconditionDef(s0);
+    assert KomUserEntryPrecondition(s0, pagedb, dispPg);
+    lemma_UserExceptionStateSideEffects(s0, s1, s3, pagedb, dispPg);
+    var pagedb' := lemma_KomUserEntryPrecond_Preserved(s0, s1, s3, pagedb, dispPg);
+    lemma_evalHandler(s3, r, pagedb', dispPg);
+}
+
+lemma lemma_PrivModeExceptionHandlersAreCorrect(s0:state, ex:exception, s1:state, r:state)
+    requires GlobalAssumptions() && ValidState(s0) && s0.ok
+        && UsermodeContinuationPrecondition(s0)
+        && priv_of_state(s0) == PL1 && interrupts_enabled(s0)
+        && (ex == ExFIQ || ex == ExIRQ)
+        && evalExceptionTaken(s0, ex, nondet_word(s0.conf.nondet, NONDET_PC()), s1)
+        && evalCode(exHandler(ex), s1, r)
+    ensures mode_of_state(s1) != User && SaneMem(s1.m)
+    ensures priv_of_mode(spsr_of_state(s1).m) == PL1
+    ensures exists p0, dp:PageNr :: KomInterruptHandlerInvariant(s1, p0, r, dp)
+{
+    var pagedb, dispPg := lemma_UsermodeContinuationPreconditionDef(s0);
+    lemma_PrivExceptionStateSideEffects(s0, s1, ex, pagedb, dispPg);
+    reveal va_eval();
+    var block := va_CCons(exHandler(ex), va_CNil());
+    assert va_eval(Block(block), s1, r) by { assert evalBlock(block, s1, r); }
+    var _, _, p := va_lemma_interrupt_handler(block, s1, r, ex, pagedb, dispPg);
+    assert KomInterruptHandlerInvariant(s1, pagedb, r, dispPg);
+}
