verified/exhandler_state.s.dfy
@@ -1,0 +1,36 @@
+include "kom_print.s.dfy"
+
+// these are global assumptions
+predicate GlobalAssumptions()
+{
+    SaneConstants()
+        && UsermodeContinuationPreconditionDef()
+        && UsermodeContinuationInvariantDef()
+        && InterruptContinuationPreconditionDef()
+        && InterruptContinuationInvariantDef()
+}
+
+// this is what we assume about the initial state on entry to the SMC handler
+predicate InitialSMCState(s:state)
+{
+    reveal ValidRegState();
+    reveal ValidSRegState();
+
+    ValidState(s) && s.ok
+        && SaneMem(s.m)
+        && mode_of_state(s) == Monitor
+        && s.conf.scr.ns == NotSecure
+        && !interrupts_enabled(s)
+        && s.regs[SP(Monitor)] == StackBase()
+        && decode_psr(s.sregs[spsr(Monitor)]).m != Monitor
+}
+
+function exHandler(ex:exception): va_code
+{
+    match ex
+        case ExAbt => abt_handler()
+        case ExUnd => und_handler()
+        case ExSVC => svc_handler()
+        case ExFIQ => fiq_handler()
+        case ExIRQ => irq_handler()
+}
