verified/kom_print.s.dfy
@@ -1,0 +1,112 @@
+include "ARMprint.s.dfy"
+include "smc_handler.gen.dfy"
+include "exception_handlers.gen.dfy"
+
+function method smc_handler():va_code  { va_code_smc_handler() }
+function method svc_handler():va_code  { va_code_svc_handler() }
+function method abt_handler():va_code  { va_code_abort_handler(ExAbt) }
+function method und_handler():va_code  { va_code_abort_handler(ExUnd) }
+function method fiq_handler():va_code  { va_code_interrupt_handler(ExFIQ) }
+function method irq_handler():va_code  { va_code_interrupt_handler(ExIRQ) }
+
+method printExceptionHandlerReturn()
+{
+    printInsFixed("B", user_continue_label());
+}
+
+method printInterruptHandlerReturn()
+{
+    printIns2Op("TST", OSP, OConst(1));
+    printInsFixed("BNE", user_continue_label());
+    printInsFixed("MOVS", "pc, lr");
+}
+
+method printSMCHandlerReturn()
+{
+    printInsFixed("MOVS", "pc, lr");
+}
+
+method printKSHA256()
+{
+    print(".type g_k_sha256, %object"); nl();
+    print(".align 5"); nl();
+    print("g_k_sha256:"); nl();
+    print(".word 0x428a2f98,0x71374491,0xb5c0fbcf,0xe9b5dba5"); nl();
+    print(".word 0x3956c25b,0x59f111f1,0x923f82a4,0xab1c5ed5"); nl();
+    print(".word 0xd807aa98,0x12835b01,0x243185be,0x550c7dc3"); nl();
+    print(".word 0x72be5d74,0x80deb1fe,0x9bdc06a7,0xc19bf174"); nl();
+    print(".word 0xe49b69c1,0xefbe4786,0x0fc19dc6,0x240ca1cc"); nl();
+    print(".word 0x2de92c6f,0x4a7484aa,0x5cb0a9dc,0x76f988da"); nl();
+    print(".word 0x983e5152,0xa831c66d,0xb00327c8,0xbf597fc7"); nl();
+    print(".word 0xc6e00bf3,0xd5a79147,0x06ca6351,0x14292967"); nl();
+    print(".word 0x27b70a85,0x2e1b2138,0x4d2c6dfc,0x53380d13"); nl();
+    print(".word 0x650a7354,0x766a0abb,0x81c2c92e,0x92722c85"); nl();
+    print(".word 0xa2bfe8a1,0xa81a664b,0xc24b8b70,0xc76c51a3"); nl();
+    print(".word 0xd192e819,0xd6990624,0xf40e3585,0x106aa070"); nl();
+    print(".word 0x19a4c116,0x1e376c08,0x2748774c,0x34b0bcb5"); nl();
+    print(".word 0x391c0cb3,0x4ed8aa4a,0x5b9cca4f,0x682e6ff3"); nl();
+    print(".word 0x748f82ee,0x78a5636f,0x84c87814,0x8cc70208"); nl();
+    print(".word 0x90befffa,0xa4506ceb,0xbef9a3f7,0xc67178f2"); nl();
+    print(".size g_k_sha256,.-g_k_sha256"); nl();
+    print(".word 0   @ terminator"); nl();
+}
+
+// TODO: clean this up (or move it to the loader)
+method printStack()
+{
+    print(".align 3"); nl(); // 8-byte alignment
+    print(".global monitor_stack_base"); nl();
+    print("monitor_stack_limit:"); nl();
+    print(".skip "); print(KOM_STACK_SIZE); nl();
+    print("monitor_stack_base:"); nl();
+}
+
+method printAll()
+{
+    var n := 0;
+    var monitor_vectbl := emptyVecTbl().(
+        svc_smc := Just("smc"),
+        fiq := Just("fiq"),
+        irq := Just("irq"));
+    var secure_vectbl := emptyVecTbl().(
+        undef := Just("undefined"),
+        svc_smc := Just("svc"),
+        prefetch_abort := Just("abort"),
+        data_abort := Just("abort"));
+
+    printHeader(); nl();
+
+    print(".section vectors, \"ax\""); nl();
+    printVecTbl("_monitor_vectors", monitor_vectbl); nl();
+    printVecTbl("_secure_vectors", secure_vectbl); nl();
+
+    nl();
+    print(".section .text"); nl();
+
+    n := printFunction("abort", abt_handler(), n);
+    printExceptionHandlerReturn(); nl();
+
+    n := printFunction("undefined", und_handler(), n);
+    printExceptionHandlerReturn(); nl();
+
+    n := printFunction("svc", svc_handler(), n);
+    printExceptionHandlerReturn(); nl();
+
+    n := printFunction("smc", smc_handler(), n);
+    printSMCHandlerReturn(); nl();
+
+    n := printFunction("fiq", fiq_handler(), n);
+    printInterruptHandlerReturn(); nl();
+
+    n := printFunction("irq", irq_handler(), n);
+    printInterruptHandlerReturn(); nl();
+
+    nl(); print(".section .data"); nl();
+    printKSHA256(); nl();
+
+    var bssglobals
+        := map o | o in KomGlobalDecls() && o != K_SHA256s() :: KomGlobalDecls()[o];
+    print(".global g_monitor_physbase, g_secure_physbase"); nl();
+    printBss(bssglobals);
+    printStack();
+}
